src/MicroSail/Iris/Model.v
@@ -216,7 +216,7 @@ Module Type IrisHeapKit
 
   Parameter Inline mem_inv_init : forall Σ (μ : Memory), memPreG Σ -> ⊢ |==> ∃ memG : memG Σ, (mem_inv memG μ ∗ mem_res memG μ)%I.
 
-  Parameter lpred_inst : forall `{sRG : sailRegG Σ} `{invG Σ} (p : 𝑷) (ts : Env Lit (𝑷_Ty p)), memG Σ -> iProp Σ.
+  Parameter luser_inst : forall `{sRG : sailRegG Σ} `{invG Σ} (p : 𝑷) (ts : Env Lit (𝑷_Ty p)), memG Σ -> iProp Σ.
 End IrisHeapKit.
 
 Module IrisInstance
@@ -392,7 +392,7 @@ Module IrisInstance
   Instance iris_IHeapLet : IHeaplet (iProp Σ) :=
     { is_ISepLogic := iris_ISepLogic;
       (* TODO: should be user-defined... *)
-      lpred p ts := lpred_inst ts sailG_memG;
+      luser p ts := luser_inst ts sailG_memG;
       lptsreg σ r t := reg_pointsTo r t
     }.
 
